verif/HMAC_top.v
@@ -1,0 +1,40 @@
+
+Require Import HMAC_specs_equiv.
+Require Import HMAC_verif.
+
+
+(*
+
+Theorem HMAC_equiv (MSGT : Set) :
+  forall keylen msglen key msg,
+    has_type key (bytestream keylen) ->
+    has_type msg (bytestream msglen) ->
+    forall c p hf res HashBlock iv (splitAndPad : MSGT -> list (Bvector (b c p))),
+      hmac_model hf key msg = Some res ->
+      @correct_model_hash c p hf (h_star p HashBlock iv) ->
+      forall nmsg nkey,
+        eappend (map bv_to_extval (splitAndPad nmsg)) = msg ->
+        bv_to_extval nkey = key ->
+        forall opad ipad,
+          same_bits 92 opad ->
+          same_bits 54 ipad ->
+          forall fpad,
+            (forall x, bv_to_extval' (app_fpad fpad (h_star p HashBlock iv x)) = bv_to_extval' (h_star p HashBlock iv x)) ->
+            eseq (bv_to_extval' (@HMAC c p HashBlock iv MSGT splitAndPad fpad opad ipad nkey nmsg)) = res.
+
+
+(* lemma for when the length of the key is the same as the length of the block *)
+Lemma Hmac_eval_keylen_is_blocklength :
+  forall (key : ext_val) keylen,
+    has_type key (bytestream keylen) -> 
+    forall GE TE SE, 
+      wf_env ge GE TE SE ->
+      (forall id, In id [(371, "ks");(372, "okey");(373, "ikey");(374, "internal")] -> GE id = None) ->
+      forall h hf,
+        good_hash h GE TE SE hf ->
+        forall msg msglen unused,
+          has_type msg (bytestream msglen) ->
+          exists v,
+            eager_eval_expr GE TE SE (apply (tapply (EVar hmac) ((typenum (Z.of_nat msglen)) :: (typenum (Z.of_nat keylen)) :: (typenum unused) :: (typenum (Z.of_nat keylen)) :: nil)) (h :: h :: h :: (EValue key) :: (EValue msg) :: nil)) (to_sval v) /\ hmac_model hf key msg = Some v.
+Proof.
+*)
